



# INDIAN INSTITUTE OF INFORMATION TECHNOLOGY, SRI CITY

## End Sem-EXAMINATION-Monsoon 2025

### Real Analysis, Numerical Analysis, and Calculus

CSE & ECE: UG2

Duration: 180 Minutes (02:30 PM-05:30 PM)

Date: 28-11-2025

Max. Marks: 45

#### Instructions:

Roll No: \_\_\_\_\_

- Marks are indicated in [ ] after each question.
- Rough work should be done separately, not with the answers.
- Answers should be reasoned and derived clearly, not a single-word answer.
- Be short and precise. Provide the answer to exactly what is asked for.
- The exam is not open book, and students are not allowed to bring textbooks, photocopies, hand-written notes, or laptops.
- Follow the instructions mentioned in the questions. Answer all the questions.
- Return the question paper and answer sheet before leaving the exam hall.
- Calculator is allowed.

1. (a) Let  $x_1 = 8$  and  $x_{n+1} = \frac{1}{2}x_n + 2$  for  $n \in \mathbb{N}$ . Show that  $(x_n)$  is bounded and monotone. Find the limit.

**Solution:** Recurrence:  $x_{n+1} = \frac{1}{2}x_n + 2$ ,  $x_1 = 8$ .

**Step 1.** Find fixed point  $L$ . Assume  $x_n \rightarrow L$ . Then

$$L = \frac{1}{2}L + 2 \Rightarrow \frac{1}{2}L = 2 \Rightarrow L = 4.$$

[1 Mark]

**Step 2.** Monotonicity. Compute

$$x_{n+1} - x_n = -\frac{1}{2}(x_n - 4).$$

If  $x_n > 4$  then  $x_{n+1} - x_n < 0$ . Since  $x_1 = 8 > 4$  and  $x_2 = \frac{1}{2} \cdot 8 + 2 = 6 > 4$ , by induction  $x_n > 4$  for all  $n$  and hence the sequence is strictly decreasing.

**Step 3.** Boundedness. Each  $x_n > 4$ , so sequence is bounded below by 4 and above by  $x_1 = 8$ .

**Conclusion.** Sequence is monotone decreasing and bounded, so it converges. Limit:

$\lim_{n \rightarrow \infty} x_n = 4.$
--

[1 Mark]

- (b) Test the convergence of the series

$$\left(\frac{1}{3}\right)^2 + \left(\frac{1 \cdot 2}{3 \cdot 5}\right)^2 + \left(\frac{1 \cdot 2 \cdot 3}{3 \cdot 5 \cdot 7}\right)^2 + \left(\frac{1 \cdot 2 \cdot 3 \cdot 4}{3 \cdot 5 \cdot 7 \cdot 9}\right)^2 + \dots$$

**Solution:** Series:

$$\left(\frac{1}{3}\right)^2 + \left(\frac{1 \cdot 2}{3 \cdot 5}\right)^2 + \left(\frac{1 \cdot 2 \cdot 3}{3 \cdot 5 \cdot 7}\right)^2 + \dots$$

Let

$$t_n = \prod_{k=1}^n \frac{k}{2k+1}, \quad a_n = t_n^2.$$

**Step 1.** Ratio for  $t_n$ :

$$\frac{t_{n+1}}{t_n} = \frac{n+1}{2n+3} \xrightarrow{n \rightarrow \infty} \frac{1}{2}.$$

[1 Mark]

**Step 2.** Ratio for  $a_n$ :

$$\frac{a_{n+1}}{a_n} = \left(\frac{t_{n+1}}{t_n}\right)^2 \rightarrow \left(\frac{1}{2}\right)^2 = \frac{1}{4} < 1.$$

**Conclusion.** By ratio test (terms decay like a geometric sequence with ratio about 1/4), the series  $\sum a_n$  converges.

The series converges.

[1 Mark]

- (c) Prove that  $\mu = \frac{2 + \Delta}{2\sqrt{1 + \Delta}}$ , where  $\Delta$  denotes the forward difference operator and  $\mu$  denotes the average operator.

**Solution:** Let  $E$  be forward shift:  $(Ef)(n) = f(n+1)$ . Then  $\Delta = E - I$  so  $1 + \Delta = E$ . Also  $2 + \Delta = I + E$ . Hence

$$\frac{2 + \Delta}{2\sqrt{1 + \Delta}} = \frac{I + E}{2E^{1/2}} = \frac{E^{-1/2} + E^{1/2}}{2},$$

which equals the average operator  $\mu$  (since  $\mu f = \frac{1}{2}(f(n) + f(n+1))$ ). Thus

$$\mu = \frac{2 + \Delta}{2\sqrt{1 + \Delta}}.$$

[1 Mark]

2. (a) Let us find an approximate solution to the nonlinear equation  $\sin x + x^2 - 1 = 0$  using regula-falsi method. Exact solution is approximately 0.637.

**Solution:**

**Step 1.** Define  $f(x) = \sin x + x^2 - 1$ . Note  $f(0) = -1 < 0$ ,  $f(1) = \sin 1 > 0$ . So a root lies in  $[0, 1]$ .

**Step 2.** Regula-falsi iteration:

$$x_{\text{new}} = b - \frac{f(b)(b-a)}{f(b) - f(a)}.$$

Start with  $a_0 = 0$ ,  $b_0 = 1$ .

**Iterations (numerical).**

$$\begin{aligned}x_1 &\approx 0.5430441252, & f(x_1) &\approx -0.1883585, \\x_2 &\approx 0.6266225471, & f(x_2) &\approx -0.0209319, \\x_3 &\approx 0.6356849974, & f(x_3) &\approx -0.0021757, \\x_4 &\approx 0.6366245537, & f(x_4) &\approx -0.0002246, \\x_5 &\approx 0.6367215023, & f(x_5) &\approx -2.316 \times 10^{-5}.\end{aligned}$$

[1Mark]

[1 Mark]

**Conclusion.** Root  $\approx 0.63672$ . Rounded to 3 decimals:

$$\boxed{x \approx 0.637.}$$

(b) Evaluate using Simpson's  $\frac{1}{3}$ rd rule  $\int_0^1 \frac{dx}{x^3 + x + 1}$ , choose step length 0.25.

Simpson's rule:  $\int_0^1 \frac{dx}{x^3 + x + 1}$  with  $h = 0.25$ .

**Solution: Step 1.** Nodes:  $x_0 = 0, x_1 = 0.25, x_2 = 0.5, x_3 = 0.75, x_4 = 1$ .

**Step 2.** Function values:

$$\begin{aligned}f(0) &= 1, \\f(0.25) &\approx 0.7901234568, \\f(0.5) &\approx 0.6153846154, \\f(0.75) &\approx 0.4604316547, \\f(1) &= \frac{1}{3}.\end{aligned}$$

[1 Mark]

**Step 3.** Composite Simpson's rule:

$$I \approx \frac{h}{3}(f_0 + 4f_1 + 2f_2 + 4f_3 + f_4) \approx \frac{0.25}{3} \cdot 7.5661 \approx 0.6305269.$$

**Conclusion.**

$$\boxed{\int_0^1 \frac{dx}{x^3 + x + 1} \approx 0.63053.}$$

[1 Mark]

3. (a) Evaluate the integral

$$\iint_{\Omega} xy \, dx \, dy,$$

where  $\Omega$  is the interior of the circle  $x^2 + y^2 \leq 1$  bounded by the straight line  $2x + y = 1$ .

**Solution: Step 1.** Find intersection points of line and circle. Solve

$$x^2 + (1 - 2x)^2 = 1 \Rightarrow 5x^2 - 4x = 0 \Rightarrow x = 0, x = \frac{4}{5}.$$

Corresponding points:  $(0, 1)$  and  $(\frac{4}{5}, -\frac{3}{5})$ .

**Step 2.** Set up integral using vertical slices for the (smaller) segment:

$$I = \int_{x=0}^{4/5} \int_{y=1-2x}^{\sqrt{1-x^2}} xy \, dy \, dx.$$

[1 Mark]

**Step 3.** Inner integral:

$$\int_{1-2x}^{\sqrt{1-x^2}} xy \, dy = x \left[ \frac{y^2}{2} \right]_{1-2x}^{\sqrt{1-x^2}} = \frac{x}{2} (1 - x^2 - (1 - 2x)^2) = \frac{x^2(4 - 5x)}{2}.$$

**Step 4.** Outer integral:

$$I = \frac{1}{2} \int_0^{4/5} (4x^2 - 5x^3) \, dx.$$

Compute:

$$\int_0^{4/5} 4x^2 \, dx = \frac{256}{375}, \quad \int_0^{4/5} 5x^3 \, dx = \frac{256}{500},$$

so

$$\int_0^{4/5} (4x^2 - 5x^3) \, dx = \frac{64}{375},$$

hence

$$I = \frac{1}{2} \cdot \frac{64}{375} = \boxed{\frac{32}{375}}.$$

[1 Mark]

(b) Let  $R = [0, 1] \times [0, 1]$  and  $f : R \rightarrow \mathbb{R}$  be defined by

$$f(x, y) = \begin{cases} 0, & \text{when } x \notin \mathbb{Q}, \\ 0, & \text{when } x \in \mathbb{Q}, y \notin \mathbb{Q}, \\ \frac{1}{q}, & \text{when } x \in \mathbb{Q}, y = \frac{p}{q} \text{ in lowest terms.} \end{cases}$$

Calculate  $\int_0^1 \int_0^1 f(x, y) \, dx \, dy$ , where  $\mathbb{Q}$  is the set of rational numbers.

**Solution:** The set where  $f \neq 0$  is contained in  $\{x \in \mathbb{Q}\} \times \{y \in \mathbb{Q}\}$ , which is countable, measure zero in  $\mathbb{R}^2$ . Hence  $f = 0$  almost everywhere and

$$\boxed{\iint_{[0,1]^2} f(x, y) \, dx \, dy = 0.}$$

[2 Mark]

(c) Find the volume of the region  $\Omega$  in  $\mathbb{R}^3$  bounded by the surfaces of the paraboloids

$$z = x^2 + y^2, \quad \text{and} \quad 2z = 12 - x^2 - y^2.$$

Volume between  $z = x^2 + y^2$  and  $2z = 12 - x^2 - y^2$ .

**Solution: Step 1.** Intersection: solve

$$x^2 + y^2 = \frac{12 - x^2 - y^2}{2} \Rightarrow x^2 + y^2 = 4.$$

So region in  $xy$ -plane is disk of radius 2.

[1 Mark]

**Step 2.** Volume:

$$V = \iint_{r \leq 2} \left( \frac{12 - r^2}{2} - r^2 \right) dA = \int_0^{2\pi} \int_0^2 \frac{12 - 3r^2}{2} r dr d\theta.$$

Inner integral evaluates to 6, so

$$V = 6 \cdot 2\pi = \boxed{12\pi}.$$

[1 Mark]

4. (a) Compute the integral

$$\iint_{\Omega} e^{\frac{y-x}{y+x}} dx dy,$$

where

$$\Omega = \{(x, y) : x \geq 0, y \geq 0, x + y \leq 1\}.$$

**Solution:** Change of variables:

$$u = y - x, \quad v = x + y.$$

Then  $x = (v - u)/2$ ,  $y = (v + u)/2$ .

**Step 2.** Jacobian:

$$\det \frac{\partial(x, y)}{\partial(u, v)} = \begin{vmatrix} -\frac{1}{2} & \frac{1}{2} \\ \frac{1}{2} & \frac{1}{2} \end{vmatrix} = \frac{1}{2}.$$

Hence  $dx dy = \frac{1}{2} du dv$ .

**Step 3.** Integrand:

$$\frac{y - x}{y + x} = \frac{u}{v}, \quad e^{(y-x)/(y+x)} = e^{u/v}.$$

**Step 4.** Region in  $(u, v)$ -plane:

$$x \geq 0 \Rightarrow v - u \geq 0 \Rightarrow u \leq v, \quad y \geq 0 \Rightarrow v + u \geq 0 \Rightarrow u \geq -v,$$

and  $0 \leq v \leq 1$ . So  $0 \leq v \leq 1$ ,  $-v \leq u \leq v$ .

[1 Mark]

**Step 5.** Integral:

$$I = \int_{v=0}^1 \int_{u=-v}^v e^{u/v} \frac{1}{2} du dv.$$

Evaluate inner integral: put  $t = u/v$ ,  $du = v dt$ ,  $t \in [-1, 1]$ :

$$\int_{-v}^v e^{u/v} du = v \int_{-1}^1 e^t dt = v(e - e^{-1}).$$

Thus

$$I = \int_0^1 \frac{1}{2} v(e - e^{-1}) dv = \frac{e - e^{-1}}{2} \cdot \frac{1}{2} = \boxed{\frac{e - e^{-1}}{4}}.$$

[1 Mark]

(b)  $\int_0^2 \int_{y/2}^1 e^{-x^2} dx dy.$

**Solution:** Region:  $0 \leq y \leq 2, y/2 \leq x \leq 1.$

Swapping order:  $0 \leq x \leq 1, 0 \leq y \leq 2x.$

$$J = \int_0^1 \int_0^{2x} e^{-x^2} dy dx = \int_0^1 2xe^{-x^2} dx.$$

[1 Mark]

Let  $u = x^2, du = 2x dx$ :

$$J = \int_0^1 e^{-u} du = 1 - e^{-1}.$$

$$\boxed{J = 1 - e^{-1}}.$$

[1 Mark]

5. (a) If  $\mathbf{F}(x, y, z) = xyz\mathbf{i} - e^z \cos x \mathbf{j} + xy^2 z^3 \mathbf{k}$ , then calculate  $\nabla \cdot (\nabla \times \mathbf{F})$ .

**Solution.** Given  $\mathbf{F} = (P, Q, R) = (xyz, -e^z \cos x, xy^2 z^3)$ .

First compute  $\nabla \times \mathbf{F}$ :

$$\nabla \times \mathbf{F} = \begin{vmatrix} \mathbf{i} & \mathbf{j} & \mathbf{k} \\ \partial_x & \partial_y & \partial_z \\ xyz & -e^z \cos x & xy^2 z^3 \end{vmatrix}.$$

Compute each component:

$$(\nabla \times \mathbf{F})_1 = \frac{\partial}{\partial y}(xy^2 z^3) - \frac{\partial}{\partial z}(-e^z \cos x) = 2xyz^3 - (-e^z \cos x) = 2xyz^3 + e^z \cos x,$$

$$(\nabla \times \mathbf{F})_2 = \frac{\partial}{\partial z}(xyz) - \frac{\partial}{\partial x}(xy^2 z^3) = xy - y^2 z^3,$$

$$(\nabla \times \mathbf{F})_3 = \frac{\partial}{\partial x}(-e^z \cos x) - \frac{\partial}{\partial y}(xyz) = e^z \sin x - xz.$$

Thus

$$\nabla \times \mathbf{F} = (2xyz^3 + e^z \cos x, xy - y^2 z^3, e^z \sin x - xz).$$

Now compute the divergence:

$$\nabla \cdot (\nabla \times \mathbf{F}) = \frac{\partial}{\partial x}(2xyz^3 + e^z \cos x) + \frac{\partial}{\partial y}(xy - y^2 z^3) + \frac{\partial}{\partial z}(e^z \sin x - xz).$$

[1 Mark]

Evaluate each derivative:

$$\frac{\partial}{\partial x}(2xyz^3 + e^z \cos x) = 2yz^3 - e^z \sin x,$$

$$\frac{\partial}{\partial y}(xy - y^2 z^3) = x - 2yz^3,$$

$$\frac{\partial}{\partial z}(e^z \sin x - xz) = e^z \sin x - x.$$

Add them:

$$(2yz^3 - e^z \sin x) + (x - 2yz^3) + (e^z \sin x - x) = 0.$$

$$\boxed{\nabla \cdot (\nabla \times \mathbf{F}) = 0.}$$

[1 Mark]

(b) Calculate the work done by the force

$$\mathbf{F} = x\mathbf{i} - y\mathbf{j} + (x + y + z)\mathbf{k}$$

on a particle that moves along the parabola  $y = 3x^2$ ,  $z = 0$  from the origin to the point  $(2, 12, 0)$ .

**Solution: Step 1.** Parameterize:  $r(t) = (t, 3t^2, 0)$ ,  $0 \leq t \leq 2$ . Then  $r'(t) = (1, 6t, 0)$ .

**Step 2.** Evaluate  $F$  on curve:

$$F(r(t)) = (t, -3t^2, t + 3t^2).$$

Dot product:

$$F \cdot r' = t - 18t^3.$$

[1 Mark]

**Step 3.** Integrate:

$$W = \int_0^2 (t - 18t^3) dt = \left[ \frac{t^2}{2} - \frac{18t^4}{4} \right]_0^2 = 2 - 72 = \boxed{-70}.$$

[1 Mark]

(c)  $\mathbf{F}(x, y, z) = xy\mathbf{i} + (xz + y)\mathbf{j} + (xy - z)\mathbf{k}$ . Find an  $f$  such that  $\nabla f = \mathbf{F}$ .

**Solution:**

$$\nabla \times F = (0, -y, z - x),$$

which is not zero in general. Therefore  $F$  is not conservative and no scalar potential  $f$  exists:

[2 Mark]

6. Let  $\mathbf{F}(x, y, z) = (xyz, y^2 + 1, z^3)$  and let  $S$  be the unit cube  $S = [0, 1] \times [0, 1] \times [0, 1]$ . Compute

$$\iint_S (\nabla \times \mathbf{F}) \cdot \mathbf{n} dS$$

using

- (a) Stokes' theorem,
- (b) the Divergence theorem.

**Solution: (a) Using Stokes' theorem.** For a closed surface  $S$  (boundary of a volume) the boundary of  $S$  is empty, so the circulation integral around  $\partial S$  is zero. Thus

$$\iint_S (\nabla \times F) \cdot n \, dS = \oint_{\partial S} F \cdot dr = 0.$$

[1 Mark]

**Solution: (b) Using divergence theorem on  $\nabla \times F$ .** Since  $\nabla \cdot (\nabla \times F) \equiv 0$ ,

$$\iint_S (\nabla \times F) \cdot n \, dS = \iiint_{[0,1]^3} \nabla \cdot (\nabla \times F) \, dV = 0.$$

[1 Mark]

Both methods give:

$$\boxed{0.}$$

7. (a) Determine the values of  $k$  for which the improper integral

$$\int_1^\infty \left( \frac{kt}{1+t^2} - \frac{1}{2t} \right) dt$$

converges.

[2 Marks]

**Solution:**

We have

$$\frac{kt}{1+t^2} - \frac{1}{2t} = \frac{(2k-1)t^2 - 1}{2t(1+t^2)}.$$

**Case 1:**  $\boxed{k \neq \frac{1}{2}}.$

For large  $t$  the dominant term in the numerator is  $(2k-1)t^2$ . Compare the integrand with  $1/t$ . Compute the limit

$$\lim_{t \rightarrow \infty} \frac{\frac{(2k-1)t^2 - 1}{2t(1+t^2)}}{1/t} = \lim_{t \rightarrow \infty} \frac{(2k-1)t^2 - 1}{2(1+t^2)} = \frac{2k-1}{2} \neq 0 \text{ and finite as } k \neq \frac{1}{2}.$$

By the Limit Comparison Test with  $g(t) = 1/t$  and using the fact that  $\int_1^\infty \frac{1}{t} dt$  diverges, we conclude that

$$\int_1^\infty \left( \frac{kt}{1+t^2} - \frac{1}{2t} \right) dt$$

diverges for every  $k \neq \frac{1}{2}$ .

[1 Mark]

**Case 2:**  $\boxed{k = \frac{1}{2}}$

If  $k = \frac{1}{2}$  the integrand becomes

$$\frac{\frac{1}{2}t}{1+t^2} - \frac{1}{2t} = -\frac{1}{2} \cdot \frac{1}{t(1+t^2)}.$$

Compare with  $g(t) = 1/t^3$ . Compute the limit

$$\lim_{t \rightarrow \infty} \frac{\frac{1}{2t(1+t^2)}}{1/t^3} = \lim_{t \rightarrow \infty} \left( -\frac{1}{2} \cdot \frac{t^3}{t(1+t^2)} \right) = \lim_{t \rightarrow \infty} \left( -\frac{1}{2} \cdot \frac{t^2}{1+t^2} \right) = -\frac{1}{2},$$



which is finite and nonzero. Since  $\int_1^\infty \frac{1}{t^3} dt$  converges, by the Limit Comparison Test the given integral converges when  $k = \frac{1}{2}$ . [1 Mark]

The improper integral  $\int_1^\infty \left( \frac{kt}{1+t^2} - \frac{1}{2t} \right) dt$  converges if and only if  $k = \frac{1}{2}$ .

(b) Consider the integral

$$\int_{-2}^1 \frac{dx}{\sqrt[3]{3x-2}}$$

(i) Identify whether this integral is **proper** or **improper**. Explain the reason.

(ii) Check whether the integral is convergent or divergent. [2 Marks]

**Solution:** This is a type II improper integral as  $y = \frac{1}{\sqrt[3]{3x-2}}$  is unbounded at

$x = \frac{2}{3}$ . [1 Mark]

We get

$$\begin{aligned} \int_{-2}^1 \frac{dx}{\sqrt[3]{3x-2}} &= \int_{-2}^{2/3} \frac{dx}{\sqrt[3]{3x-2}} + \int_{2/3}^1 \frac{dx}{\sqrt[3]{3x-2}} \\ &= \lim_{b \rightarrow 2/3^-} \int_{-2}^b \frac{dx}{\sqrt[3]{3x-2}} + \lim_{a \rightarrow 2/3^+} \int_a^1 \frac{dx}{\sqrt[3]{3x-2}} \\ &= \lim_{b \rightarrow 2/3^-} \left[ \frac{(3x-2)^{2/3}}{2} \right]_{-2}^b + \lim_{a \rightarrow 2/3^+} \left[ \frac{(3x-2)^{2/3}}{2} \right]_a^1 \\ &= \lim_{b \rightarrow 2/3^-} \left( \frac{(3b-2)^{2/3}}{2} - 2 \right) + \lim_{a \rightarrow 2/3^+} \left( 1 - \frac{(3a-2)^{2/3}}{2} \right) \\ &= (0 - 2) + (1 - 0) \\ &= \boxed{-1}. \end{aligned}$$

[1 Mark]

8. (a) Show that  $\Gamma\left(\frac{1}{2} + x\right) \Gamma\left(\frac{1}{2} - x\right) = \pi \sec(\pi x)$ .

**Solution:**

$$\begin{aligned} \Gamma\left(\frac{1}{2} + x\right) \Gamma\left(\frac{1}{2} - x\right) &= \Gamma\left(\frac{1+2x}{2}\right) \Gamma\left(\frac{1-2x}{2}\right) \\ &= \Gamma\left(1 - \frac{1-2x}{2}\right) \Gamma\left(\frac{1-2x}{2}\right) \\ &= \frac{\pi}{\sin\left\{\pi\left(\frac{1-2x}{2}\right)\right\}} \\ &= \frac{\pi}{\sin\left(\frac{\pi}{2} - \pi x\right)} \\ &= \frac{\pi}{\cos(\pi x)} \\ &= \pi \sec(\pi x). \end{aligned}$$

[1 Mark]

[1 Mark]

(b) Evaluate

$$\int_0^\infty \frac{x^3(1+x^4)}{(1+x)^{12}} dt$$

using gamma and beta functions.

[2 Marks]

**Solution:**

$$\begin{aligned} \int_0^\infty \frac{x^3(1+x^4)}{(1+x)^{12}} dx &= \int_0^\infty \frac{x^3}{(1+x)^{12}} dx + \int_0^\infty \frac{x^7}{(1+x)^{12}} dx \\ &= \int_0^\infty \frac{x^{4-1}}{(1+x)^{4+8}} dx + \int_0^\infty \frac{x^{8-1}}{(1+x)^{8+4}} dx \\ &= B(4, 8) + B(8, 4) \\ &= 2B(4, 8) \quad [\because B(m, n) = B(n, m)] \\ &= 2 \left[ \frac{\Gamma(4)\Gamma(8)}{\Gamma(4+8)} \right] \quad \left[ \because B(m, n) = \frac{\Gamma(m)\Gamma(n)}{\Gamma(m+n)} \right] \\ &= 2 \left[ \frac{3!7!}{11!} \right] \\ &= \frac{1}{660}. \end{aligned}$$

[1 Mark]

[1 Mark]

9. (a) State whether the following statement is **True** or **False**, and explain why.

“ There exists a function  $f : \mathbb{R}^2 \rightarrow \mathbb{R}$  such that  $\frac{\partial f}{\partial x} = y$  and  $\frac{\partial f}{\partial y} = x^2$ .”

**Solution:** FALSE

If there were such a function, then its mixed second partial derivatives would be

$$\frac{\partial^2 f}{\partial y \partial x} = 1 \quad \text{and} \quad \frac{\partial^2 f}{\partial x \partial y} = 2x.$$

These functions are continuous and unequal. But we know that if a function has continuous mixed second partial derivatives then it must be equal.

[1 Mark]

- (b) Let  $u = x^2 - 2y^2, v = 2x^2 - y^2$  with  $x = r \cos \theta, y = r \sin \theta$ . Show that  $\frac{\partial(u, v)}{\partial(r, \theta)} = 6r^3 \sin 2\theta$ .

[1 Mark]

**Solution:**

$$\begin{aligned} x &= r \cos \theta, & y &= r \sin \theta, \\ u &= x^2 - 2y^2 = r^2(\cos^2 \theta - 2\sin^2 \theta), & v &= 2x^2 - y^2 = r^2(2\cos^2 \theta - \sin^2 \theta), \\ \frac{\partial u}{\partial r} &= 2r(\cos^2 \theta - 2\sin^2 \theta), & \frac{\partial u}{\partial \theta} &= -6r^2 \sin \theta \cos \theta, \\ \frac{\partial v}{\partial r} &= 2r(2\cos^2 \theta - \sin^2 \theta), & \frac{\partial v}{\partial \theta} &= -2r^2 \sin \theta \cos \theta, \end{aligned}$$

[  $\frac{1}{2}$  Mark]

$$\begin{aligned}\frac{\partial(u, v)}{\partial(r, \theta)} &= \begin{vmatrix} \frac{\partial u}{\partial r} & \frac{\partial u}{\partial \theta} \\ \frac{\partial v}{\partial r} & \frac{\partial v}{\partial \theta} \end{vmatrix} \\ &= \begin{vmatrix} 2r(\cos^2 \theta - 2 \sin^2 \theta) & -6r^2 \sin \theta \cos \theta \\ 2r(2 \cos^2 \theta - \sin^2 \theta) & -2r^2 \sin \theta \cos \theta \end{vmatrix} \\ &= 6r^3 \sin 2\theta.\end{aligned}$$

[  $\frac{1}{2}$  Mark]

(c) Consider

$$f(x, y) = \begin{cases} \frac{x^2 y}{x^2 + y^2}, & (x, y) \neq (0, 0), \\ 0, & (x, y) = (0, 0). \end{cases}$$

(i) Is  $f$  continuous at  $(0, 0)$ ?

(ii) Compute  $\frac{\partial f}{\partial x}$  and  $\frac{\partial f}{\partial y}$ . Are these continuous at  $(0, 0)$ ?

(iii) Is  $f$  differentiable at  $(0, 0)$ ?

[3 Marks]

**Solution: (a) Continuity at  $(0, 0)$ .**

For  $(x, y) \neq (0, 0)$ ,

$$|f(x, y)| = \left| \frac{x^2 y}{x^2 + y^2} \right| = \frac{x^2}{x^2 + y^2} |y| \leq |y| \leq \sqrt{x^2 + y^2}.$$

Given  $\varepsilon > 0$ , choose  $\delta = \varepsilon$ . If  $\sqrt{x^2 + y^2} < \delta$ , then

$$|f(x, y) - 0| = |f(x, y)| \leq \sqrt{x^2 + y^2} < \delta = \varepsilon.$$

Hence

$$\boxed{f \text{ is continuous at } (0, 0).}$$

[1 Mark]

**(b) Compute  $\partial f / \partial x$  and  $\partial f / \partial y$  and check continuity.**

For  $(x, y) \neq (0, 0)$ ,

$$f_x(x, y) = \frac{2xy(x^2 + y^2) - 2xx^2y}{(x^2 + y^2)^2} = \frac{2xy^3}{(x^2 + y^2)^2}.$$

At  $(0, 0)$ ,

$$f_x(0, 0) = \lim_{h \rightarrow 0} \frac{f(h, 0) - 0}{h} = 0.$$

Along  $y = x$ ,

$$f_x(x, x) = \frac{2x \cdot x^3}{(2x^2)^2} = \frac{1}{2} \neq 0.$$

Thus

$$\boxed{f_x \text{ is not continuous at } (0, 0).}$$

[  $\frac{1}{2}$  Mark]

For  $(x, y) \neq (0, 0)$ ,

$$f_y(x, y) = \frac{x^2(x^2 + y^2) - 2yx^2y}{(x^2 + y^2)^2} = \frac{x^2(x^2 - y^2)}{(x^2 + y^2)^2}.$$

At  $(0, 0)$ ,

$$f_y(0, 0) = \lim_{h \rightarrow 0} \frac{f(0, h) - 0}{h} = 0.$$

Along  $y = x^2$ ,

$$f_y(x, x^2) = \frac{1 - x^2}{(1 + x^2)^2} \rightarrow 1 \neq 0.$$

Thus

$f_y$  is not continuous at  $(0, 0)$ .

[  $\frac{1}{2}$  Mark]

**(c) Differentiability at  $(0, 0)$**

$f$  is differentiable at  $(0, 0)$  iff

$$\lim_{(h,k) \rightarrow (0,0)} \frac{f(h, k) - 0 - 0 - 0}{\sqrt{h^2 + k^2}} = \lim_{(h,k) \rightarrow (0,0)} \frac{h^2k}{(h^2 + k^2)^{3/2}} = 0.$$

Take the path  $k = h$ :

$$\frac{h^2h}{(h^2 + h^2)^{3/2}} = \frac{h^3}{(2h^2)^{3/2}} = \frac{1}{2\sqrt{2}} \neq 0.$$

Therefore the required limit does not exist, so

$f$  is not differentiable at  $(0, 0)$ .

[1 Mark]

10. (a) Find the critical points of  $f(x, y) = x^2 + xy + y^2 + \frac{1}{x} + \frac{1}{y}$ .

[1 Mark]

**Solution** Given

$$f(x, y) = x^2 + xy + y^2 + \frac{1}{x} + \frac{1}{y}.$$

We have

$$\frac{\partial f}{\partial x} = 2x + y - \frac{1}{x^2}, \quad \frac{\partial f}{\partial y} = x + 2y - \frac{1}{y^2}.$$

To find critical points:

$$2x + y - \frac{1}{x^2} = 0 \Rightarrow 2x^3 + x^2y - 1 = 0, \quad (1)$$

$$x + 2y - \frac{1}{y^2} = 0, \Rightarrow xy^2 + 2y^3 - 1 = 0. \quad (2)$$

[  $\frac{1}{2}$  Mark]

$$\begin{aligned} (1) - (2) &\Rightarrow (2x^3 + x^2y - 1) - (xy^2 + 2y^3 - 1) = 0, \\ &\Rightarrow 2(x^3 - y^3) + xy(x - y) = 0, \\ &\Rightarrow (x - y)(2(x^2 + xy + y^2) + xy) = 0, \\ &\Rightarrow (x - y)(2x^2 + 3xy + 2y^2) = 0. \end{aligned}$$

Hence

$$x - y = 0 \Rightarrow x = y.$$

Substitute  $x = y$  into (1) (or (2)):

$$2x + x - \frac{1}{x^2} = 0 \Rightarrow 3x - \frac{1}{x^2} = 0,$$

so

$$3x = \frac{1}{x^2} \Rightarrow x^3 = \frac{1}{3}.$$

Therefore the critical point is  $((1/3)^{1/3}, (1/3)^{1/3})$ . [  $\frac{1}{2}$  Mark]

(b) Show that the rectangular solid of maximum volume that can be inscribed in a sphere is a cube. [2 Marks]

**Solution:** Let  $2x, 2y, 2z$  be the length, breadth and height of the rectangular solid. Then its volume is  $V = 8xyz$ .

Let the sphere have a radius of  $r$  so that  $x^2 + y^2 + z^2 = r^2$ .

Taking  $F(x, y, z) = V + \lambda(x^2 + y^2 + z^2 - r^2) = 8xyz + \lambda(x^2 + y^2 + z^2 - r^2)$ , where  $\lambda$  is the multiplier.

$$\frac{\partial F}{\partial x} = 8yz + 2\lambda x = 0 \tag{1}$$

$$\frac{\partial F}{\partial y} = 8xz + 2\lambda y = 0 \tag{2}$$

$$\frac{\partial F}{\partial z} = 8xy + 2\lambda z = 0 \tag{3}$$

Multiplying (1), (2), (3) by  $x, y, z$  respectively, we get:

$$8xyz + 2\lambda x^2 = 0 \tag{4}$$

$$8xyz + 2\lambda y^2 = 0 \tag{5}$$

$$8xyz + 2\lambda z^2 = 0 \tag{6}$$

From (4), (5), (6) we have  $x^2 = y^2 = z^2$ . Since  $x, y, z > 0$ , we conclude  $x = y = z$ .

Thus the rectangular solid is a cube. [1 Mark]